theories/Session.v
@@ -1,0 +1,214 @@
+From mathcomp.ssreflect Require Import all_ssreflect seq.
+From mathcomp Require Import finmap.
+Set Implicit Arguments.
+Unset Strict Implicit.
+Import Prenex Implicits.
+
+Require Import MPST.Atom.
+Require Import MPST.Role.
+Require Import MPST.Forall.
+Require Import MPST.LNVar.
+Require Import MPST.Actions.
+
+Section Session.
+
+  Inductive s_ty :=
+  | s_end
+  | s_var (v : rvar)
+  | s_rec (S : s_ty)
+  | s_msg (a: l_act) (K : seq (lbl * (mty * s_ty))).
+
+  Open Scope mpst_scope.
+
+  Fixpoint eq_sty x y :=
+    match x, y with
+    | s_end, s_end => true
+    | s_var x, s_var y => x == y
+    | s_rec x, s_rec y => eq_sty x y
+    | s_msg a1 Ks1, s_msg a2 Ks2
+      => (a1 == a2)
+           && (fix eqK Ks1 Ks2 :=
+                 match Ks1, Ks2 with
+                 | [::], [::] => true
+                 | K1::Ks1, K2::Ks2 =>
+                   (K1.lbl == K2.lbl)
+                     && (K1.mty == K2.mty)
+                     && eq_sty K1.cnt K2.cnt && eqK Ks1 Ks2
+                 | _, _ => false
+                 end) Ks1 Ks2
+    (* all2 (fun l r => (l.1 == r.1) && eq_lty l.2 r.2) K1 K2 *)
+    | _, _ => false
+    end.
+
+  Definition eq_salt (l r : lbl * (mty * s_ty)) :=
+    (l.lbl == r.lbl) && (l.mty == r.mty) && eq_sty l.cnt r.cnt.
+
+  Lemma eq_smsg_all a1 a2 K1 K2 :
+    eq_sty (s_msg a1 K1) (s_msg a2 K2) = (a1 == a2) && all2 eq_salt K1 K2.
+  Proof.
+    rewrite /=; case: eqP=>[/=_{a1 a2}|//]; move: K1 K2.
+    by elim=>//[[l1 [t1 L1]] K1] Ih; case=>//[[l2 [t2 L2]] K2]/=; rewrite Ih.
+  Qed.
+
+  Lemma sty_eqP : Equality.axiom eq_sty.
+  Proof.
+    rewrite /Equality.axiom; fix Ih 1 => x y.
+    case: x => [|v|L|a K];
+       case: y =>[|v'|L'|a' K']; try (by constructor).
+    + by rewrite /eq_sty; case: eqP=>[->|F]; constructor=>//[[/F]].
+    + by rewrite /=; case: Ih=>[->|F]; constructor=>//[[/F]].
+    + rewrite eq_smsg_all/=; case: eqP=>[<-{a'}|F]/=; [|by constructor=>[[/F]]].
+      elim: K K'=>[|[l [t L]] K IhK]; case=>[|[l' [t' L']]K']/=; try (by constructor).
+      rewrite {1}/eq_salt/=; do 2 (case: eqP=>[<-|F];[|constructor=>[[/F]]//]).
+      case: Ih=>[<-|F];[|constructor=>[[/F]]//].
+      by case: IhK=>[[]<-|F]; constructor=>//[[]]H; apply: F; rewrite H.
+  Qed.
+
+  Definition sty_eqMixin := EqMixin sty_eqP.
+  Canonical sty_eqType := Eval hnf in EqType s_ty sty_eqMixin.
+
+  Fixpoint s_open (d : nat) (S2 : s_ty) (S1 : s_ty) :=
+    match S1 with
+    | s_end => S1
+    | s_var v => Rvar.open s_var d S2 v
+    | s_rec s => s_rec (s_open d.+1 S2 s)
+    | s_msg a K => s_msg a [seq (lS.lbl, (lS.mty, s_open d S2 lS.cnt)) | lS <- K]
+    end.
+  Notation sfv a := (s_var (Rvar.fv a)).
+  Notation sbv n := (s_var (Rvar.bv n)).
+  Notation "{ k '~>' v } s":= (s_open k v s) (at level 30, right associativity).
+  Notation "L '^' v":= (s_open 0 (sfv v) L) (at level 30, right associativity).
+
+  Fixpoint s_close (v : atom) (d : nat) (L1 : s_ty) :=
+    match L1 with
+    | s_end => L1
+    | s_var lv => s_var (Rvar.close v d lv)
+    | s_rec L => s_rec (s_close v d.+1 L)
+    | s_msg a K => s_msg a [seq (lL.lbl, (lL.mty, s_close v d lL.cnt)) | lL <- K]
+    end.
+  Notation "{ k '<~' v } L":= (s_close v k L) (at level 30, right associativity).
+
+  Fixpoint s_fvar (L : s_ty) : {fset atom} :=
+    match L with
+    | s_end => fset0
+    | s_var v => Rvar.fvar v
+    | s_rec L => s_fvar L
+    | s_msg _ K => fsetUs [seq s_fvar lL.cnt | lL <- K]
+    end.
+
+  Fixpoint s_fbvar (d : nat) (L : s_ty) : {fset nat} :=
+    match L with
+    | s_end => fset0
+    | s_var v => Rvar.fbvar d v
+    | s_rec L => s_fbvar d.+1 L
+    | s_msg _ K => fsetUs [seq s_fbvar d lL.cnt | lL <- K]
+    end.
+
+  Lemma sty_ind :
+    forall (P : s_ty -> Prop),
+      P s_end ->
+      (forall v, P (s_var v)) ->
+      (forall s, P s -> P (s_rec s)) ->
+      (forall a K, Forall (fun lS => P lS.cnt) K -> P (s_msg a K)) ->
+      forall s : s_ty, P s.
+  Proof.
+    move => P P_end P_var P_rec P_msg.
+    fix Ih 1; case=>[|v|L|a K].
+    + by apply: P_end.
+    + by apply: P_var.
+    + by apply: P_rec.
+    + by apply: P_msg; elim: K.
+  Qed.
+
+  Lemma s_open_close X L n : X \notin s_fvar L -> {n <~ X}{n ~> sfv X}L = L.
+  Proof.
+    elim/sty_ind: L n=>[|v|L Ih|a K Ih] n /=Fv//;
+      try (by rewrite Ih).
+    + by move: Fv; rewrite Rvar.open_fun/= =>H; rewrite Rvar.open_close.
+    + move: Ih=>/Fa_lift/(_ n)-Ih; move: Fv => /notin_unions/Fa_map-Fv.
+      move: (Fa_app (Fa_conj Ih Fv)) => {Ih Fv}Ih; rewrite -map_comp /comp/=.
+      by elim: K Ih=>// [[l [t L]] K Ih/= [-> /Ih-[->]]].
+  Qed.
+
+  Lemma s_close_open n X L : n \notin s_fbvar 0 L -> {n ~> sfv X}{n <~ X}L = L.
+  Proof.
+    move: {1 3}n (add0n n)=>n0; elim/sty_ind: L 0 n =>///=.
+    - by move=>v n n1;rewrite addnC Rvar.open_fun=><-H;rewrite Rvar.close_open.
+    - by move=>G Ih n n1 Eq/= H; rewrite (Ih n.+1 n1.+1) // -Eq.
+    - move=> a K /Fa_lift-Ih n n1 Eq /notin_unions/Fa_map-H.
+      move:Ih=>/(_ n)/Fa_lift/(_ n1)/Fa_lift/(_ Eq)/Fa_conj/( _ H)/Fa_app-Ih{H}.
+      congr s_msg; rewrite -map_comp/comp/=; elim: K Ih=>[//|[l[t S]] K Ih /=].
+      by move=>[->/Ih->].
+  Qed.
+
+  Fixpoint depth_sty L :=
+    match L with
+    | s_end
+    | s_var _ => 0
+    | s_rec L => (depth_sty L).+1
+    | s_msg _ K  => (maximum [seq depth_sty l.cnt | l <- K]).+1
+    end.
+
+  Lemma s_depth_open L X : depth_sty L = depth_sty (L^X).
+  Proof.
+    move: 0; elim/sty_ind: L=>/=//.
+    + by move=>v n; rewrite Rvar.open_fun.
+    + by move=> L Ih n; rewrite (Ih n.+1).
+    + move=> a K Ih n; rewrite -map_comp /comp/=.
+      by move: Ih => /Fa_lift/(_ n)/Fa_map_eq<-.
+  Qed.
+
+  Lemma sty_ind1 :
+    forall (P : s_ty -> Prop),
+      P s_end ->
+      (forall v, P (s_var v)) ->
+      (forall s, (forall X (A : {fset atom}), X \notin A -> P (s ^ X)) ->
+                 P (s_rec s)) ->
+      (forall a Ks, (forall K, K \in Ks -> P K.cnt) -> P (s_msg a Ks)) ->
+      forall s : s_ty, P s.
+  Proof.
+    move => P P_end P_var P_rec P_msg L.
+    move: {-1}(depth_sty L) (leqnn (depth_sty L))=> n; move: n L; elim.
+    + by case.
+    + move=>n Ih; case=>/=//.
+      - by move=>L D; apply:P_rec=>X S _;apply: Ih;rewrite -(s_depth_open L X).
+      - move=> a K D;apply: P_msg =>L /(map_f (fun X => depth_sty X.cnt)).
+        move=>/in_maximum_leq-/=dG; move: (leq_trans dG D)=>{dG} {D}.
+        by apply: Ih.
+  Qed.
+
+  Fixpoint dual (L : s_ty) : s_ty :=
+    match L with
+    | s_end => s_end
+    | s_var v => s_var v
+    | s_rec s => s_rec (dual s)
+    | s_msg a K => s_msg (dual_act a) [seq (x.lbl, (x.mty, dual x.cnt)) | x <- K]
+    end.
+
+  Lemma dualK s : dual (dual s) = s.
+  Proof.
+    elim/sty_ind: s=>[|v|s Ih|a K Ih]//; try (by rewrite /=Ih).
+    - rewrite /= -map_comp /comp/= dual_actK.
+      by elim: K Ih=>[//|[l [t s]] K Ihl /= [-> /Ihl-[->]]].
+  Qed.
+
+  Definition is_dual (s1 s2 : s_ty) : bool := s1 == dual s2.
+
+  Lemma isdual_sym (s1 s2 : s_ty) : is_dual s1 s2 -> is_dual s2 s1.
+  Proof. by move=>/eqP->; rewrite /is_dual dualK. Qed.
+
+  Lemma is_dual_var v : is_dual (s_var v) (s_var v).
+  Proof. by rewrite /is_dual/dual. Qed.
+
+  Lemma isdualC (s1 s2 : s_ty) : is_dual s1 s2 = is_dual s2 s1.
+  Proof.
+    move: {-1}(is_dual s1 s2) (eq_refl (is_dual s1 s2)) => D.
+    rewrite /is_dual; case: D=>[/eqP/eqP->|].
+    - by rewrite dualK eq_refl.
+    - move=>/eqP; rewrite (rwP negPf)=> H; apply/esym; move: H; apply: contraTF.
+      by rewrite negbK=>/eqP->; rewrite dualK.
+  Qed.
+
+  Lemma dualI : injective dual.
+  Proof. by move=>x1 x2; rewrite -{2}(dualK x1) -{2}(dualK x2)=>->. Qed.
+End Session.
