theories/TraceEquiv.v
@@ -110,6 +110,9 @@ Section TraceEquiv.
     | _, _ => None
     end.
 
+  Print l_ty.
+
+
   Fail Inductive mq_proj p : rg_ty -> MsgQ -> l_ty -> Prop :=
   | prj_end :
       mq_proj p rg_end [::] l_end
